src/lowparse/pulse/LowParse.Pulse.Int.fst
@@ -40,6 +40,31 @@ inline_for_extraction
 let read_u8 : reader serialize_u8 = reader_of_leaf_reader (read_u8' ())
 
 inline_for_extraction
+let size_u8 (#t: Type) (vmatch: t -> FStar.UInt8.t -> slprop) : compute_remaining_size vmatch serialize_u8 =
+  compute_remaining_size_constant_size vmatch serialize_u8 1sz
+
+inline_for_extraction
+noextract
+[@@FStar.Tactics.postprocess_with (fun _ -> FStar.Tactics.norm [delta_attr [`%E.must_reduce]; iota; zeta; primops]; FStar.Tactics.trefl ())]
+let n_to_be_1 =  (E.mk_n_to_be EI.uint8 1)
+
+inline_for_extraction
+```pulse
+fn l2r_leaf_write_u8 (_: unit) : l2r_leaf_writer u#0 #FStar.UInt8.t #parse_u8_kind #parse_u8 serialize_u8
+= (n: _)
+  (x: _)
+  (pos: SZ.t)
+  (#v: Ghost.erased (Seq.seq byte))
+{
+  S.pts_to_len x;
+  serialize_u8_spec_be n;
+  let pos' = SZ.add pos 1sz;
+  n_to_be_1 n x pos';
+  pos'
+}
+```
+
+inline_for_extraction
 let validate_u16 : validator parse_u16 =
   validate_total_constant_size parse_u16 2sz
 
@@ -69,6 +94,31 @@ fn read_u16' (_: unit) : leaf_reader #FStar.UInt16.t #parse_u16_kind #parse_u16 
 
 inline_for_extraction
 let read_u16 : reader serialize_u16 = reader_of_leaf_reader (read_u16' ())
+
+inline_for_extraction
+let size_u16 (#t: Type) (vmatch: t -> FStar.UInt16.t -> slprop) : compute_remaining_size vmatch serialize_u16 =
+  compute_remaining_size_constant_size vmatch serialize_u16 2sz
+
+inline_for_extraction
+noextract
+[@@FStar.Tactics.postprocess_with (fun _ -> FStar.Tactics.norm [delta_attr [`%E.must_reduce]; iota; zeta; primops]; FStar.Tactics.trefl ())]
+let n_to_be_2 =  (E.mk_n_to_be EI.uint16 2)
+
+inline_for_extraction
+```pulse
+fn l2r_leaf_write_u16 (_: unit) : l2r_leaf_writer u#0 #FStar.UInt16.t #parse_u16_kind #parse_u16 serialize_u16
+= (n: _)
+  (x: _)
+  (pos: SZ.t)
+  (#v: Ghost.erased (Seq.seq byte))
+{
+  S.pts_to_len x;
+  serialize_u16_spec_be n;
+  let pos' = SZ.add pos 2sz;
+  n_to_be_2 n x pos';
+  pos'
+}
+```
 
 inline_for_extraction
 let validate_u32 : validator parse_u32 =
@@ -102,6 +152,31 @@ inline_for_extraction
 let read_u32 : reader serialize_u32 = reader_of_leaf_reader (read_u32' ())
 
 inline_for_extraction
+let size_u32 (#t: Type) (vmatch: t -> FStar.UInt32.t -> slprop) : compute_remaining_size vmatch serialize_u32 =
+  compute_remaining_size_constant_size vmatch serialize_u32 4sz
+
+inline_for_extraction
+noextract
+[@@FStar.Tactics.postprocess_with (fun _ -> FStar.Tactics.norm [delta_attr [`%E.must_reduce]; iota; zeta; primops]; FStar.Tactics.trefl ())]
+let n_to_be_4 =  (E.mk_n_to_be EI.uint32 4)
+
+inline_for_extraction
+```pulse
+fn l2r_leaf_write_u32 (_: unit) : l2r_leaf_writer u#0 #FStar.UInt32.t #parse_u32_kind #parse_u32 serialize_u32
+= (n: _)
+  (x: _)
+  (pos: SZ.t)
+  (#v: Ghost.erased (Seq.seq byte))
+{
+  S.pts_to_len x;
+  serialize_u32_spec_be n;
+  let pos' = SZ.add pos 4sz;
+  n_to_be_4 n x pos';
+  pos'
+}
+```
+
+inline_for_extraction
 let validate_u64 : validator parse_u64 =
   validate_total_constant_size parse_u64 8sz
 
@@ -131,3 +206,28 @@ fn read_u64' (_: unit) : leaf_reader #FStar.UInt64.t #parse_u64_kind #parse_u64 
 
 inline_for_extraction
 let read_u64 : reader serialize_u64 = reader_of_leaf_reader (read_u64' ())
+
+inline_for_extraction
+let size_u64 (#t: Type) (vmatch: t -> FStar.UInt64.t -> slprop) : compute_remaining_size vmatch serialize_u64 =
+  compute_remaining_size_constant_size vmatch serialize_u64 8sz
+
+inline_for_extraction
+noextract
+[@@FStar.Tactics.postprocess_with (fun _ -> FStar.Tactics.norm [delta_attr [`%E.must_reduce]; iota; zeta; primops]; FStar.Tactics.trefl ())]
+let n_to_be_8 =  (E.mk_n_to_be EI.uint64 8)
+
+inline_for_extraction
+```pulse
+fn l2r_leaf_write_u64 (_: unit) : l2r_leaf_writer u#0 #FStar.UInt64.t #parse_u64_kind #parse_u64 serialize_u64
+= (n: _)
+  (x: _)
+  (pos: SZ.t)
+  (#v: Ghost.erased (Seq.seq byte))
+{
+  S.pts_to_len x;
+  serialize_u64_spec_be n;
+  let pos' = SZ.add pos 8sz;
+  n_to_be_8 n x pos';
+  pos'
+}
+```
